l-expressions i

An L-expression is defined as any one of the following:

a natural number;
the symbol $A$;
the symbol $Z$;
the symbol $S$;
a pair of L-expressions $u, v$, which is written as $u(v)$.


An L-expression can be transformed according to the following rules:

$A(x) \to x + 1$ for any natural number $x$;
$Z(u)(v) \to v$ for any L-expressions $u, v$;
$S(u)(v)(w) \to v(u(v)(w))$ for any L-expressions $u, v, w$.


For example, after applying all possible rules, the L-expression $S(Z)(A)(0)$ is transformed to the number $1$:
$$S(Z)(A)(0) \to A(Z(A)(0)) \to A(0) \to 1.$$
Similarly, the L-expression $S(S)(S(S))(S(Z))(A)(0)$ is transformed to the number $6$ after applying all possible rules.

Find the result of the L-expression $S(S)(S(S))(S(S))(S(Z))(A)(0)$ after applying all possible rules. Give the last nine digits as your answer.
Note: it can be proved that the L-expression in question can only be transformed a finite number of times, and the final result does not depend on the order of the transformations.